examples/webmodel/OAuth.IP.fst
@@ -1,3 +1,6 @@
+(*
+  Defines the functionality of the IP in the OAuth protocol
+*)
 module OAuth.IP
 
 open FStar.All
@@ -18,6 +21,9 @@ open OAuth.Datatypes
 let ipurl = ({c_origin=ipori;c_uname=emptyString (SecretVal [ipori]);c_pwd=emptyString (SecretVal [ipori]);c_path=[];c_querystring=[];c_fragment=emptyString (SecretVal [ipori])})
 let ipuri = mk_uri ipurl
 
+type uList = (list (secString (SecretVal [ipori]) * secString (SecretVal [ipori]) * list (secString (SecretVal [ipori]))))
+let userList:uList = [((classify #PublicVal "usernameU" (SecretVal [ipori])), (classify #PublicVal "passwordP" (SecretVal [ipori])), [])]
+
 val checkIPReq : req:request -> Tot (b:bool)
 let checkIPReq req =
   match (Request?.rsl req) with
@@ -34,46 +40,40 @@ let rec isValid #l ls s =
     | [] -> false
     | hd::tl -> eqString (hd) s || isValid tl s
   
-val isValidSessionId : #l:secLevel -> uList l -> string -> Tot bool
-let rec isValidSessionId #l sl s = 
+val isValidSessionId : uList -> string -> Tot bool
+let rec isValidSessionId sl s = 
   match sl with
     | [] -> false
     | (_,_,c)::tl -> isValid c s || isValidSessionId tl s 
 
 (* check the validity of the password *)
-val isValidPwd : #l:secLevel -> #l':secLevel -> uList (SecretVal [ipori]) -> (secString l) -> (secString l') -> Tot bool
+val isValidPwd : #l:secLevel -> #l':secLevel -> uList -> (secString l) -> (secString l') -> Tot bool
 let rec isValidPwd #l #l' sl su sp = 
   match sl with
     | [] -> false
     | (u,p,_)::tl -> if (s_equal u su) then (s_equal p sp) else isValidPwd tl su sp 
     
-val isAlreadyLoggedIn : uList (SecretVal [ipori]) -> list (string * string) -> Tot bool
+val isAlreadyLoggedIn : uList -> list (string * string) -> Tot bool
 let isAlreadyLoggedIn ul l = isValidSessionId ul (getVal #PublicVal l "_ipsid")
 
-val authenticateUser : uList (SecretVal [ipori]) -> req:request -> Tot bool
+val authenticateUser : uList -> req:request -> Tot bool
 let authenticateUser ul req =
   let s = (s_getRequestBody #(Request?.rsl req) req) in
   let qs = getFormData s in
   isValidPwd ul (getQSVal qs "user") (getQSVal qs "pwd")
-		    
-(* authentication of the user - return the authcode along with the state to the RP *)
-val getIPAuthResp : r:request -> ML (resp:actResponse{requestResponseValid r resp})
-let getIPAuthResp r =
-    let rsl = s_getReqURISecLevel r in
-    let ruri = s_getRequestURI r in
-    let ul = !userList in 
-    if ((isAlreadyLoggedIn ul (getReqCookie (s_getReqHeaderValue r "Cookie"))) ||
-       ((Request?.rf r).reqm = "POST" && (authenticateUser ul r))) then
-       let cid = declassify (getQSVal ruri.c_querystring "client_id") in
-       let reduri = s_secstring_uri #PublicVal (declassify (getQSVal ruri.c_querystring "redirect_uri")) in 
-       match reduri with 
-       | None -> (print_string ("Error:getIPAuthResp - getRPOrigin \n");defErrResponse)
-       | Some (o,red) -> (* && (getRPOrigin cid = (s_getURI (Some?.v reduri)).c_origin) ) then ( check for origins to be the same? *)
+
+val ipAuthResp : #rsl:secLevel -> ruri:c_uri rsl -> r:request{Request?.rsl r = rsl} -> ML (resp:actResponse{requestResponseValid r resp})
+let ipAuthResp #rsl ruri r =
+  let cid = declassify (getQSVal ruri.c_querystring "client_id") in
+  let reduri = s_secstring_uri #PublicVal (declassify (getQSVal ruri.c_querystring "redirect_uri")) in 
+  match reduri with 
+  | None -> (print_string ("Error:getIPAuthResp - getRPOrigin \n");defErrResponse)
+  | Some (o,red) -> (* && (getRPOrigin cid = (s_getURI (Some?.v reduri)).c_origin) ) then ( check for origins to be the same? *)
 	 let urisl = SecretVal [o] in
-	 let rori = declassify (getQSVal #rsl ruri.c_querystring "origin") in
+	 (* let rori = declassify (getQSVal #rsl ruri.c_querystring "origin") in *)
 	 let token = classify #PublicVal (declassify (getQSVal #rsl ruri.c_querystring "csrftoken")) urisl in
 	 let authcode = genSecret urisl in
-	 let ipREP = curi_to_hstring ({c_origin=red.c_origin;c_uname=classify red.c_uname urisl;c_pwd=classify red.c_pwd urisl;c_path=classifyPath red.c_path urisl;c_querystring=[(classify #PublicVal "authcode" urisl, getSecret (authcode));(classify #PublicVal "csrftoken" urisl, token);(classify #PublicVal "IP" urisl,classify #PublicVal (origin_to_string ipori) urisl)];c_fragment=emptyString urisl}) in
+	 let ipREP = curi_to_hstring ({c_origin=red.c_origin;c_uname=classify red.c_uname urisl;c_pwd=classify red.c_pwd urisl;c_path=classifyPath red.c_path urisl;c_querystring=[(classify #PublicVal "authcode" urisl, getSecret (authcode));(classify #PublicVal "csrftoken" urisl, token);(classify #PublicVal "Issuer" urisl,classify #PublicVal (origin_to_string ipori) urisl)];c_fragment=emptyString urisl}) in
 	 let stateToken = Secret urisl token in 
 	 let rduri = mk_uri red in 
 	 ipCL := (o, stateToken, authcode, rduri)::(!ipCL);
@@ -83,11 +83,21 @@ let getIPAuthResp r =
 	 let chead = (if (emptyList (getReqCookie (s_getReqHeaderValue r "Cookie"))) then [("Set-Cookie", (mk_svheaderval ck))] else []) in
 	 let nhead = ("Location", (mk_headerval #urisl ipREP))::chead in
 	 ActResponse (SecretVal [o;ipori]) ({resptype="default";respcode=303;respurl=[];resphead=nhead;respbody=(emptyString (SecretVal [o;ipori]));resptrail=[];respHTTPS="modern";respCSP=cspPol;respCORS=[];resploc=None;respRedSec=urisl})
-	 )	 
+	 )
+	 
+(* authentication of the user - return the authcode along with the state to the RP *)
+val getIPAuthResp : r:request -> ML (resp:actResponse{requestResponseValid r resp})
+let getIPAuthResp r =
+    let rsl = s_getReqURISecLevel r in
+    let ruri = s_getRequestURI r in
+    let ul = userList in 
+    if ((isAlreadyLoggedIn ul (getReqCookie (s_getReqHeaderValue r "Cookie"))) ||
+       ((Request?.rf r).reqm = "POST" && (authenticateUser ul r))) then
+       ipAuthResp #rsl ruri r	 
     else if ((Request?.rf r).reqm = "GET") then (* send login form for authentication *)
     (
        let cid = declassify (getQSVal ruri.c_querystring "client_id") in
-       if (getRPOrigin cid = s_getRequestOrigin r) then 
+       if (getRPOrigin (Secret PublicVal cid) = s_getRequestOrigin r) then 
 	 ActResponse (SecretVal [ipori]) ({resptype="default";respcode=200;respurl=[];resphead=[];respbody=(emptyString (SecretVal [ipori]));resptrail=[];respHTTPS="modern";respCSP=cspPol;respCORS=[];resploc=None;respRedSec=PublicVal})
        else
 	 defErrResponse
@@ -102,7 +112,7 @@ let getIPTokenResp r =
     let ruri = s_getRequestURI r in
     let cid = declassify (getQSVal ruri.c_querystring "client_id") in
     let reduri = secstring_to_uri #urisl (getQSVal ruri.c_querystring "redirect_uri") in
-    let rorig = getRPOrigin cid in
+    let rorig = getRPOrigin (Secret PublicVal cid) in
     let olist = (SecretVal [ipori;rorig]) in
     let cs = (getQSVal ruri.c_querystring "client_secret") in
     let code = (getQSVal ruri.c_querystring "authcode") in
@@ -125,7 +135,7 @@ let getIPTokenResp r =
 	   else
 	      defErrResponse)
 
-val ipReqResp : req:request -> ML (ret:retReqResp{isValidRetResp req ret /\ (RetResponse? ret)})
+val ipReqResp : r:request -> ML (ret:retReqResp{isValidRetResp r ret /\ (RetResponse? ret)})
 let ipReqResp r =
     let urisl = s_getReqURISecLevel r in
     let ruri = s_getRequestURI #urisl r in (* get the request url *)
