examples/webmodel/OAuth.RP.fst
@@ -1,3 +1,6 @@
+(*
+  Defines the functionality of the RP in the OAuth protocol
+*)
 module OAuth.RP
 
 open FStar.All
@@ -27,16 +30,17 @@ let checkRPReq req =
 val rpReqLemma : req:request -> Lemma (requires (checkRPReq req)) (ensures (restricts (Request?.rsl req) (SecretVal [rpori]))) [SMTPat (checkRPReq req)]
 let rpReqLemma req = ()
 
-(* use a browser for sending request containing authcode from RP to IP at the end of the protocol *)
-let rpb = ST.alloc (init_browser)
-let irp = match (set_unique_id !rpb) with | (f, s) -> rpb := s; f (* Get a unique_id (f) and browser (s) *)
-let rpdoc = {dloc=rpuri;dref=blank_uri;dori=(mk_aorigin rpurl.c_origin);dHTTPS="none";drefPol=RP_OriginWhenCO;dCSP=[];dsbox=[];}
-(* create a window in the browser to send the request with "rpdoc" as the document *)
-let rpsw = 
-      let hist = HistEntry (URI?.usl rpuri) (URI?.u rpuri) get_time rpdoc irp in 
-      let newwin = (win_to_cowin ({winid=irp;wname="";wloc=rpuri;wframes=[];wopener=None;wparent=None;whist={hlhe=[hist];hcur=1};wdoc=(rpdoc);wsbox=[];})) in
-      (rpb := ({(!rpb) with windows=newwin::(!rpb).windows})); newwin
+(* (\* use a browser for sending request containing authcode from RP to IP at the end of the protocol *\) *)
+let rpbr :ref browser = ST.alloc (init_browser) 
+(* let irp = match (set_unique_id !rpb) with | (f, s) -> rpb := s; f (\* Get a unique_id (f) and browser (s) *\) *)
+(* let rpdoc = {dloc=rpuri;dref=blank_uri;dori=(mk_aorigin rpurl.c_origin);dHTTPS="none";drefPol=RP_OriginWhenCO;dCSP=[];dsbox=[];} *)
+(* (\* create a window in the browser to send the request with "rpdoc" as the document *\) *)
+(* let rpsw =  *)
+(*       let hist = HistEntry (URI?.usl rpuri) (URI?.u rpuri) get_time rpdoc irp in  *)
+(*       let newwin = (win_to_cowin ({winid=irp;wname="";wloc=rpuri;wframes=[];wopener=None;wparent=None;whist={hlhe=[hist];hcur=1};wdoc=(rpdoc);wsbox=[];})) in *)
+(*       (rpb := ({(!rpb) with windows=newwin::(!rpb).windows})); newwin *)
 
+(* send the initial login request to the IP *)
 val rpLoginIPAuth : r:request -> ML (resp:actResponse{requestResponseValid r resp}) 
 let rpLoginIPAuth r =
   let urisl = s_getReqURISecLevel r in
@@ -48,8 +52,11 @@ let rpLoginIPAuth r =
     let sl = (SecretVal [rpori;ipori]) in 
     let sid = (genSecret sl) in
     let state = (genSecret sl) in 
-    let cid = (getRPClientID ipori) in
+    match (getRPClientID ipori) with
+    | None -> (print_string ("Error: Client id not found\n" ); (defErrResponse))
+    | Some clid ->
     (
+      let cid = declassify #PublicVal (getSecret clid) in 
       (let logsession:loginSession = [(ipori, sid, state)] in
       rpLS := List.append logsession (!rpLS));
       let respuri = ({c_origin=ipori;c_uname=emptyString sl;c_pwd=emptyString sl;c_path=[classify #PublicVal "authEP" sl];c_querystring=[(classify #PublicVal "client_id" sl,classify #PublicVal cid sl);(classify #PublicVal "redirect_uri" sl, classify #PublicVal "https://rp.com:443/codeEP/" sl);(classify #PublicVal "origin" sl, classify #PublicVal "https://rp.com:443/" sl);(classify #PublicVal "csrftoken" sl,getSecret state)];c_fragment=emptyString sl}) in
@@ -62,15 +69,19 @@ let rpLoginIPAuth r =
     let sl = (SecretVal [rpori;badipori]) in
     let sid = (genSecret sl) in
     let state = (genSecret sl) in
+    match (getRPClientID ipori) with (* getting ipori's client_id as the badip will replace it eventually *)
+    | None -> (print_string ("Error: Client id not found\n" ); (defErrResponse))
+    | Some clid ->
     (
+      let cid = declassify #PublicVal (getSecret clid) in 
       (let logsession:loginSession = [(badipori, sid, state)] in
       rpLS := List.append logsession (!rpLS));
       (* Badip replaces the response headers as per its convenience - the badip can modify the origin-index also  *)
       let usl = (SecretVal [rpori;ipori]) in
-      let respuri = ({c_origin=ipori;c_uname="";c_pwd="";c_path=["authEP"];c_querystring=[("client_id",(getRPClientID ipori));("redirect_uri","https://rp.com:443/codeEP/");("origin","https://rp.com/");("csrftoken",declassify #sl (getSecret state))];c_fragment=""}) in
+      let respuri = ({c_origin=ipori;c_uname="";c_pwd="";c_path=["authEP"];c_querystring=[("client_id",cid);("redirect_uri","https://rp.com:443/codeEP/");("origin","https://rp.com/");("csrftoken",declassify #sl (getSecret state))];c_fragment=""}) in
       let rpREP = classify #PublicVal (curi_to_hstring respuri) usl in
       let rpResp = ActResponse usl ({resptype="default";respcode=301;respurl=[]; resphead=[("Set-Cookie", (mk_headerval (classify #PublicVal (declassify #sl (getSecret sid)) usl)));("Location", (mk_headerval rpREP))]; respbody=(emptyString usl);resptrail=[];respHTTPS="modern";respCSP=cspPol;respCORS=[];resploc=None;respRedSec=usl}) in
-      (* print_string ("IP is not ip.com:" ^ (curi_to_hstring respuri) ^ "\n" );  *)
+      print_string ("IP is not ip.com:" ^ (curi_to_hstring respuri) ^ "\n" );
       (rpResp)
       ))
   else (print_string ("IP is not ip.com:" ^ (declassify ip) ^ "\n" ); (defErrResponse))
@@ -79,40 +90,54 @@ val getRPLoginIPAuth : r:request -> ML (ret:retReqResp{isValidRetResp r ret})
 let getRPLoginIPAuth r = (let resp = rpLoginIPAuth r in RetResponse resp)
 
 (* Compact authcode resend method for the RP *)
-val rpReqCodeEP : request -> ML (option (r:request{notForbiddenHeaderfieldInReqHeader (Request?.rf r).reqhead}))
-let rpReqCodeEP r =
+val rpReqCodeEP : request -> browser -> cowindow ->  ML (option (r:request{notForbiddenHeaderfieldInReqHeader (Request?.rf r).reqhead}))
+let rpReqCodeEP r rpb rpsw =
   let urisl = s_getReqURISecLevel r in
   let ruri = mk_uri (s_getRequestURI #urisl r) in (* get the request url *)
   let qs = getQS #urisl (ruri) in
   let csrftoken = mk_secretval (getQSVal #urisl qs "csrftoken") in
+  let actualIP = mk_secretval (getQSVal #urisl qs "Issuer") in
   let ip = getIPLogin !rpLS csrftoken in (* determine the IP based on the state-token *)
   if (ip = blank_origin) then 
     (None)
-  else
+  else if ((declassify #urisl (getSecret actualIP)) = (origin_to_string ip)) then 
+    (print_string ("Actual IP: " ^ (declassify #urisl (getSecret actualIP)) ^ "\nMy IP: " ^ (origin_to_string ip));
     let urisl = SecretVal [ip] in
     let code = declassify (getQSVal #(URI?.usl ruri) qs "authcode") in
-    let cid = (getRPClientID ip) in
-    (match (getCDSecret (!rpCD) ip) with
-    | None -> (* get client data secret is none for the ip -- may be the client_secret was not established *)
+    match (getRPClientID ip) with 
+    | None -> (print_string ("Error: Client id not found with req-code\n" ); None)
+    | Some clid ->
+	let cid = declassify #PublicVal (getSecret clid) in 
+	(match (getCDSecret (!rpCD) ip) with
+	| None -> (* get client data secret is none for the ip -- may be the client_secret was not established *)
 	   (
 	   (* The port is required to pass isOriginSec in StringFunctions *)
 	   let rturi = ({c_origin=ip;c_uname=emptyString urisl;c_pwd=emptyString urisl;c_path=[(classify #PublicVal "tokenEP" urisl)];c_querystring=[((classify #PublicVal "client_id" urisl), classify #PublicVal cid urisl);((classify #PublicVal "redirect_uri" urisl),(classify #PublicVal "https://rp.com:443/codeEP/" urisl));((classify #PublicVal "authcode" urisl),(classify #PublicVal code urisl))];c_fragment=emptyString urisl}) in
 	   let nreq = Request urisl ({reqm = "POST"; requrl = [(mk_uri rturi)]; reqhead = []; reqo = mk_aorigin ((URI?.u (CWindow?.cwloc rpsw)).c_origin); reqw = (Some rpsw); reqinit = ""; reqtype = ""; reqdest = ""; reqtarget = None; reqredirect = 0; reqredmode = "follow"; reqref = (Client rpsw); reqrefPolicy = RP_OriginWhenCO; reqnonce = ""; reqparser = ""; requnsafe = false; reqpreflight = false; reqsync = false; reqmode = NoCORS; reqtaint = "basic"; reqcredm = "omit"; reqcredflag = false; reqbody = (emptyString urisl); corsflag = false; corspfflag = false; authflag = false; recflag = false}) in
-	   let (r, req, tw, nb) = navigateWindow !rpb rpsw rpsw (RequestResource nreq) "other" in
-	   rpb := nb; (req)
+	   let (r, req, tw, nb) = navigateWindow rpb rpsw rpsw (RequestResource nreq) "other" in
+	   rpbr := nb; (req)
 	   )
-    | Some sec ->
+	| Some sec ->
 	   (
 	   secretOriginLemma ip (Secret?.s sec);
 	   let cs = classify #(Secret?.s sec) (getSecret #(Secret?.s sec) (sec)) urisl in
 	   let rturi = ({c_origin=ip;c_uname=emptyString urisl;c_pwd=emptyString urisl;c_path=[(classify #PublicVal "tokenEP" urisl)];c_querystring=[((classify #PublicVal "client_id" urisl), classify #PublicVal cid urisl);((classify #PublicVal "redirect_uri" urisl),(classify #PublicVal "https://rp.com:443/codeEP/" urisl));((classify #PublicVal "authcode" urisl),(classify #PublicVal code urisl));((classify #PublicVal "client_secret" urisl),cs)];c_fragment=emptyString urisl}) in
 	   let nreq = Request urisl ({reqm = "POST"; requrl = [(mk_uri rturi)]; reqhead = []; reqo = mk_aorigin ((URI?.u (CWindow?.cwloc rpsw)).c_origin); reqw = (Some rpsw); reqinit = ""; reqtype = ""; reqdest = ""; reqtarget = None; reqredirect = 0; reqredmode = "follow"; reqref = (Client rpsw); reqrefPolicy = RP_OriginWhenCO; reqnonce = ""; reqparser = ""; requnsafe = false; reqpreflight = false; reqsync = false; reqmode = NoCORS; reqtaint = "basic"; reqcredm = "omit"; reqcredflag = false; reqbody = (emptyString urisl); corsflag = false; corspfflag = false; authflag = false; recflag = false}) in
-	   let (r, req, tw, nb) = navigateWindow !rpb rpsw rpsw (RequestResource nreq) "other" in
-	   rpb := nb; (req)
-	   ))
+	   let (r, req, tw, nb) = navigateWindow rpb rpsw rpsw (RequestResource nreq) "other" in
+	   rpbr := nb; (req)
+	   )))
+  else (print_string ("Error: The IP does not match\n"); None)
 
 val getRPReqCodeEP : r:request -> ML (ret:retReqResp{isValidRetResp r ret})
-let getRPReqCodeEP r = (match rpReqCodeEP r with | None -> RetResponse defErrResponse | Some req -> RetRequest req)
+let getRPReqCodeEP r = 
+  (* use a browser for sending request containing authcode from RP to IP at the end of the protocol *)
+  let rpb = (init_browser) in
+  let (irp, sb) = (set_unique_id rpb) in  (* Get a unique_id (f) and browser (s) *)
+  let rpdoc = ({dloc=rpuri;dref=blank_uri;dori=(mk_aorigin rpurl.c_origin);dHTTPS="none";drefPol=RP_OriginWhenCO;dCSP=[];dsbox=[];}) in
+   (* create a window in the browser to send the request with "rpdoc" as the document *)
+  let hist = (HistEntry (URI?.usl rpuri) (URI?.u rpuri) get_time rpdoc irp) in 
+  let newwin = (win_to_cowin ({winid=irp;wname="";wloc=rpuri;wframes=[];wopener=None;wparent=None;whist={hlhe=[hist];hcur=1};wdoc=(rpdoc);wsbox=[];})) in
+  (match rpReqCodeEP r ({(sb) with windows=newwin::(sb).windows}) newwin with | None -> RetResponse defErrResponse | Some req -> RetRequest req)
 
 (* For different requests, return different responses *)
 val rpReqResp : r:request -> ML (ret:retReqResp{isValidRetResp r ret})
